Flushed out set_certificate_chain and moved it to tls_wrapper.dfy

Helpers/Structs.dfy
@@ -3,6 +3,37 @@ include "Constants.dfy"
 module Structs {
     import opened Constants
 
+    class Socket
+  {
+    var keySize : int;
+    var privateKey : string;
+    var remHostname : string;
+    var alpnProtos : array<string>;
+    var cipherSuites : array<SSL_CIPHER?>;
+
+    method Init(kSize : int, pKey : string, rHostname : string)
+      modifies this
+      ensures fresh(alpnProtos)
+      ensures fresh(cipherSuites)
+      ensures keySize == kSize
+      ensures privateKey == pKey
+      ensures remHostname == rHostname
+    {
+      keySize := kSize;
+      privateKey := pKey;
+      remHostname := rHostname;
+      alpnProtos := new string[maxSize];
+      cipherSuites := new SSL_CIPHER?[maxSize];
+    }
+
+
+    predicate Secure()
+      reads this
+    {
+      1 == 1
+    }
+  }
+
     class SSL_CTX {
         var cert_chain : array<string>;
         var x509 : string;
@@ -17,7 +48,7 @@ module Structs {
             cert_chain := new string[maxSize];
 
             // this is what SSl_CTX_new sets when it is called, resources are freed when this is 0
-            reference_count := 1; 
+            reference_count := 1;
         }
 
         predicate Valid()
