verify.dfy
@@ -5,57 +5,24 @@ module verify {
   import opened Constants
   import opened Structs
 
-  class Socket
-  {
-    var keySize : int;
-    var privateKey : string;
-    var remHostname : string;
-    var alpnProtos : array<string>;
-    var cipherSuites : array<SSL_CIPHER?>;
-
-    method Init(kSize : int, pKey : string, rHostname : string)
-      modifies this
-      ensures fresh(alpnProtos)
-      ensures fresh(cipherSuites)
-      ensures keySize == kSize
-      ensures privateKey == pKey
-      ensures remHostname == rHostname
-    {
-      keySize := kSize;
-      privateKey := pKey;
-      remHostname := rHostname;
-      alpnProtos := new string[maxSize];
-      cipherSuites := new SSL_CIPHER?[maxSize];
-    }
-
-
-    predicate Secure()
-      reads this
-    {
-      1 == 1
-    }
-  }
-
+module main{
+  import opened Structs
   method main()
-  {
-    var sock := new Socket;
-    var privateKey := "privateKey";
-    var hostname := "hostname";
+    {
+      var sock := new Socket;
+      var privateKey := "privateKey";
+      var hostname := "hostname";
 
-    sock.Init(256, privateKey, hostname);
-    // assert all properties
-    assert sock.keySize == 256;
-    assert sock.privateKey == "privateKey";
-    assert sock.remHostname == hostname;
-    assert fresh(sock.alpnProtos);
-    assert fresh(sock.cipherSuites);
-    
+      sock.Init(256, privateKey, hostname);
+      // assert all properties
+      assert sock.keySize == 256;
+      assert sock.privateKey == "privateKey";
+      assert sock.remHostname == hostname;
+      assert fresh(sock.alpnProtos);
+      assert fresh(sock.cipherSuites);
 
-    assert sock.Secure();
+
+      assert sock.Secure();
+    }
   }
 }
-
-
-
-
-
